Changes to composition theorem in symbolic execution, bespoke compsets, clean-up of definitions

hol/p4_exec_semScript.sml
@@ -9,43 +9,43 @@ open p4Theory p4_auxTheory;
 (*********************************)
 (* Expression-related shorthands *)
 
-Definition is_v:
+Definition is_v_def:
  (is_v (e_v v) = T) /\
  (is_v _ = F)
 End
 
-Definition get_v:
+Definition get_v_def:
  (get_v (e_v v) = SOME v) /\
  (get_v _ = NONE)
 End
 
-Definition is_v_bool:
+Definition is_v_bool_def:
  (is_v_bool (e_v (v_bool b)) = T) /\
  (is_v_bool _ = F)
 End
 
-Definition is_v_bit:
+Definition is_v_bit_def:
  (is_v_bit (e_v (v_bit bitv)) = T) /\
  (is_v_bit _ = F)
 End
 
 (* NOTE: Error messages serialised using 32 bits *)
-Definition is_v_err:
+Definition is_v_err_def:
  (is_v_err (e_v (v_bit (bl, 32))) = T) /\
  (is_v_err _ = F)
 End
 
-Definition is_v_str:
+Definition is_v_str_def:
  (is_v_str (e_v (v_str x)) = T) /\
  (is_v_str _ = F)
 End
 
-Definition is_var:
+Definition is_var_def:
  (is_var (e_var x) = T) /\
  (is_var _ = F)
 End
 
-Definition unop_exec:
+Definition unop_exec_def:
  (unop_exec unop_neg (v_bool b) = SOME (v_bool ~b))
  /\
  (unop_exec unop_compl (v_bit bitv) = SOME (v_bit (bitv_bl_unop bnot bitv)))
@@ -57,13 +57,13 @@ Definition unop_exec:
  (unop_exec unop v = NONE)
 End
 
-Definition e_exec_unop:
+Definition e_exec_unop_def:
  (e_exec_unop unop (e_v v) = unop_exec unop v)
   /\
  (e_exec_unop _ _ = NONE)
 End
 
-Definition cast_exec:
+Definition cast_exec_def:
  (cast_exec cast (v_bit bitv) = SOME (v_bit $ bitv_cast cast bitv))
  /\
  (cast_exec cast (v_bool b) = SOME (v_bit $ bool_cast cast b))
@@ -71,14 +71,14 @@ Definition cast_exec:
  (cast_exec cast v = NONE)
 End
 
-Definition e_exec_cast:
+Definition e_exec_cast_def:
  (e_exec_cast (cast_unsigned n) (e_v v) = cast_exec n v)
   /\
  (e_exec_cast _ _ = NONE)
 End
 
 (* TODO: Split binop into binop, binpred, ... to reduce copypaste? *)
-Definition binop_exec:
+Definition binop_exec_def:
  (binop_exec binop_mul (v_bit bitv1) (v_bit bitv2) =
   case bitv_binop binop_mul bitv1 bitv2 of
   | SOME bitv3 => SOME (v_bit bitv3)
@@ -166,13 +166,13 @@ Definition binop_exec:
  (binop_exec binop v1 v2 = NONE)
 End
 
-Definition e_exec_binop:
+Definition e_exec_binop_def:
  (e_exec_binop (e_v v1) binop (e_v v2) = binop_exec binop v1 v2)
   /\
  (e_exec_binop _ _ _ = NONE)
 End
 
-Definition e_exec_short_circuit:
+Definition e_exec_short_circuit_def:
  (e_exec_short_circuit (v_bool T) binop_bin_and e = SOME e)
   /\
  (e_exec_short_circuit (v_bool F) binop_bin_and e = SOME (e_v (v_bool F)))
@@ -185,7 +185,7 @@ Definition e_exec_short_circuit:
 End
 
 (* Field access *)
-Definition e_exec_acc:
+Definition e_exec_acc_def:
  (e_exec_acc (e_acc (e_v (v_struct f_v_list)) f) =
   case FIND (\(k, v). k = f) f_v_list of
   | SOME (f, v) => SOME (e_v v)
@@ -199,7 +199,7 @@ Definition e_exec_acc:
  (e_exec_acc _ = NONE)
 End
 
-Definition e_exec_select:
+Definition e_exec_select_def:
  (e_exec_select (e_v v) s_l_x_l x =
   case v of
   | v_struct x_v_l =>
@@ -210,14 +210,14 @@ Definition e_exec_select:
  (e_exec_select _ _ _ = NONE)
 End
 
-Definition e_exec_concat:
+Definition e_exec_concat_def:
  (e_exec_concat (e_v (v_bit bitv1)) (e_v (v_bit bitv2)) =
   SOME (v_bit (bitv_concat bitv1 bitv2)))
   /\
  (e_exec_concat _ _ = NONE)
 End
 
-Definition e_exec_slice:
+Definition e_exec_slice_def:
  (e_exec_slice (e_v (v_bit bitv1)) (e_v (v_bit bitv2)) (e_v (v_bit bitv3)) =
   SOME (v_bit (slice bitv1 bitv2 bitv3)))
   /\
@@ -227,40 +227,40 @@ End
 (********************************)
 (* Statement-related shorthands *)
 
-Definition is_empty:
+Definition is_empty_def:
  (is_empty stmt_empty = T) /\
  (is_empty _ = F)
 End
 
-Definition is_empty_singleton:
+Definition is_empty_singleton_def:
  (is_empty_singleton [stmt_empty] = T) /\
  (is_empty_singleton _ = F)
 End
 
-Definition get_ret_v:
+Definition get_ret_v_def:
  (get_ret_v (stmt_ret (e_v v)) = SOME v) /\
  (get_ret_v (stmt_seq (stmt_ret (e_v v)) stmt) = SOME v) /\
  (get_ret_v _ = NONE)
 End
 
-Definition stmt_exec_ass:
+Definition stmt_exec_ass_def:
  (stmt_exec_ass lval (e_v v) ss =
   assign ss v lval)
   /\
  (stmt_exec_ass _ _ _ = NONE)
 End
 
-Definition stmt_exec_init:
+Definition stmt_exec_init_def:
  (stmt_exec_init varn (e_v v) ss = initialise ss varn v)
 End
 
-Definition stmt_exec_trans:
+Definition stmt_exec_trans_def:
  (stmt_exec_trans (e_v (v_str x)) = SOME (status_trans x))
   /\
  (stmt_exec_trans _ = NONE)
 End
 
-Definition stmt_exec_cond:
+Definition stmt_exec_cond_def:
  (stmt_exec_cond (e_v (v_bool T)) =
   SOME T)
   /\
@@ -270,9 +270,9 @@ Definition stmt_exec_cond:
  (stmt_exec_cond _ = NONE)
 End
 
-val e_state_size_def = Define `
+Definition e_state_size_def:
  (e_state_size ((ctx:'a ctx), (g_scope_list:g_scope_list), (scope_list:scope_list), (e:e)) = e_size e)
-`;
+End
 
 (* TODO: Write explicit NONE-reducing clauses for operands of wrong types?
  *       This would reduce warnings *)
@@ -496,12 +496,7 @@ Cases_on `h` >> (
 fs [v_of_e_def]
 QED
 
-(*
-Defn.tgoal $ Hol_defn "stmt_exec"
-
-Define `
-*)
-Definition stmt_exec:
+Definition stmt_exec_def:
  (******************************************)
  (* Catch-all clauses for special statuses *)
  (stmt_exec (ctx:'a ctx) ((ascope:'a, g_scope_list:g_scope_list, frame_list:frame_list, status_returnv v):'a state) = NONE)
@@ -669,7 +664,6 @@ Definition stmt_exec:
   /\
  (stmt_exec _ _ = NONE)
 End
-(* ` *)
 
 Theorem exec_stmt_SOME_init_running:
 !ctx ascope ascope' g_scope_list g_scope_list' funn stmt frame_list' scope_list status status'.
@@ -682,7 +676,7 @@ Cases_on `stmt` >> (
  fs []
 ) >> (
  Cases_on `status` >> (
-  fs [stmt_exec]
+  fs [stmt_exec_def]
  )
 )
 QED
@@ -1084,7 +1078,7 @@ stmt_exec ctx (ascope, g_scope_list, [(funn, (stmt_ass lval e)::stmt_stack, scop
 Proof
 rpt strip_tac >>
 Cases_on `scope_list` >> Cases_on `stmt_stack` >> (
- fs [stmt_exec]
+ fs [stmt_exec_def]
 ) >>
 Cases_on `is_v e` >> (
  fs []
@@ -1147,7 +1141,7 @@ stmt_exec ctx (ascope, g_scope_list, [(funn, (stmt_trans e)::stmt_stack, scope_l
 Proof
 rpt strip_tac >>
 Cases_on `scope_list` >> Cases_on `stmt_stack` >> Cases_on `is_v e` >> (
- fs [stmt_exec]
+ fs [stmt_exec_def]
 ) >| [
  (* TODO: Not needed? *)
  Cases_on `is_v_str e` >> (
@@ -1209,7 +1203,7 @@ stmt_exec ctx (ascope, g_scope_list, [(funn, (stmt_cond e stmt1 stmt2)::stmt_sta
 Proof
 rpt strip_tac >>
 Cases_on `scope_list` >> Cases_on `stmt_stack` >> Cases_on `is_v_bool e` >> (
- fs [stmt_exec]
+ fs [stmt_exec_def]
 ) >| [
  Cases_on `stmt_exec_cond e` >> (
   fs []
@@ -1275,7 +1269,7 @@ stmt_exec (apply_table_f, ext_map, func_map, b_func_map, pars_map, tbl_map) (asc
 Proof
 rpt strip_tac >>
 Cases_on `scope_list` >> Cases_on `stmt_stack` >> Cases_on `index_not_const e_l` >> (
- fs [stmt_exec]
+ fs [stmt_exec_def]
 ) >| [
  Cases_on `ALOOKUP tbl_map t_name` >> (
   fs []
@@ -1348,7 +1342,7 @@ stmt_exec ctx (ascope, g_scope_list, [(funn, (stmt_ret e)::stmt_stack, scope_lis
 Proof
 rpt strip_tac >>
 Cases_on `scope_list` >> Cases_on `stmt_stack` >> Cases_on `get_v e` >> (
- fs [stmt_exec]
+ fs [stmt_exec_def]
 ) >| [
  Cases_on `e_exec ctx g_scope_list (h::t) e` >> (
   fs []
@@ -1392,7 +1386,7 @@ stmt_exec (apply_table_f, ext_map, func_map, b_func_map, pars_map, tbl_map) (asc
 Proof
 rpt strip_tac >>
 Cases_on `scope_list` >> Cases_on `stmt_stack` >> (
- fs [stmt_exec]
+ fs [stmt_exec_def]
 ) >| [
  Cases_on `lookup_ext_fun funn ext_map` >> (
   fs []
@@ -1428,7 +1422,7 @@ stmt_exec ctx (ascope, g_scope_list, [(funn, (stmt_block decl_list stmt)::stmt_s
 Proof
 rpt strip_tac >>
 Cases_on `scope_list` >> Cases_on `stmt_stack` >> (
- fs [stmt_exec]
+ fs [stmt_exec_def]
 ) >> (
  metis_tac []
 )
@@ -1479,7 +1473,7 @@ Cases_on `stmt` >> (
  Cases_on `stmt_stack` >> (
   fs []
  ) >>
- fs [stmt_exec] >>
+ fs [stmt_exec_def] >>
  Cases_on `is_empty s` >> (
   fs []
  ) >>
@@ -1635,7 +1629,7 @@ rpt strip_tac >| [
 
  (* Extern *)
  rename1 `[(funn,[stmt_ext],scope::scope_list)]` >>
- fs [stmt_exec] >>
+ fs [stmt_exec_def] >>
  Cases_on `lookup_ext_fun funn ext_map` >> (
   fs []
  ) >>
@@ -1686,20 +1680,20 @@ rpt strip_tac >| [
   fs [exec_stmt_app_SOME_REWRS]
  ),
 
- fs [stmt_exec],
+ fs [stmt_exec_def],
 
  (* Block entry *)
  fs [exec_stmt_block_SOME_REWRS],
 
- fs [stmt_exec],
+ fs [stmt_exec_def],
 
  (* Block exit *)
- fs [stmt_exec] >>
+ fs [stmt_exec_def] >>
  Cases_on `stmt_stack` >> (
   fs []
  ),
 
- fs [stmt_exec],
+ fs [stmt_exec_def],
 
  (* Assign *)
  fs [exec_stmt_ass_SOME_REWRS] >>
@@ -1719,7 +1713,7 @@ rpt strip_tac >| [
  fs [exec_stmt_ext_SOME_REWRS],
 
  (* Seq *)
- fs [stmt_exec] >>
+ fs [stmt_exec_def] >>
  Cases_on `is_empty stmt1` >> (
   fs []
  ) >>
@@ -1780,13 +1774,13 @@ rpt strip_tac >| [
   fs []
  ) >>
  IMP_RES_TAC stmt_exec_block >>
- fs [stmt_exec],
+ fs [stmt_exec_def],
 
  (* Initial trans status *)
- fs [stmt_exec],
+ fs [stmt_exec_def],
 
  (* Initial return status *)
- fs [stmt_exec],
+ fs [stmt_exec_def],
 
  fs [],
 
@@ -1839,7 +1833,7 @@ stmt_exec ctx (ascope, g_scope_list, [(funn, (stmt_seq stmt1 stmt2)::stmt_stack,
 Proof
 rpt strip_tac >>
 Cases_on `scope_list` >> Cases_on `stmt_stack` >> Cases_on `is_empty stmt1` >> (
- fs [stmt_exec]
+ fs [stmt_exec_def]
 ) >| [
  metis_tac [],
 
@@ -2042,7 +2036,7 @@ Proof
 Induct_on ‘stmt’ >- (
  rpt strip_tac >>
  Cases_on ‘scope_list’ >> (
-  fs[stmt_exec]
+  fs[stmt_exec_def]
  )
 ) >- (
  fs[exec_stmt_ass_SOME_REWRS]
@@ -2123,21 +2117,21 @@ rpt strip_tac >| [
  rename1 `(apply_table_f, ext_map, func_map, b_func_map, pars_map, tbl_map)` >>
  fs [exec_stmt_app_SOME_REWRS],
 
- fs [stmt_exec],
+ fs [stmt_exec_def],
 
  fs [exec_stmt_block_SOME_REWRS],
 
- fs [stmt_exec] >>
+ fs [stmt_exec_def] >>
  Cases_on `stmt_stack` >> (
   fs []
  ),
 
- fs [stmt_exec] >>
+ fs [stmt_exec_def] >>
  Cases_on `stmt_stack` >> (
   fs []
  ),
 
- fs [stmt_exec],
+ fs [stmt_exec_def],
 
  fs [exec_stmt_ass_SOME_REWRS],
 
@@ -2161,7 +2155,7 @@ rpt strip_tac >| [
   Cases_on `is_empty stmt1` >> (
    fs []
   ) >| [
-   fs [stmt_exec],
+   fs [stmt_exec_def],
 
    fs [exec_stmt_seq_SOME_REWRS]
   ]
@@ -2183,9 +2177,9 @@ rpt strip_tac >| [
   gs []
  ),
 
- fs [stmt_exec],
+ fs [stmt_exec_def],
 
- fs [stmt_exec],
+ fs [stmt_exec_def],
 
  fs [],
 
@@ -2196,7 +2190,7 @@ QED
 (* Then, define an executable semantics which performs execution until out of fuel. *)
 (* Note that all concrete operations remain the same *)
 (* Note that expression multi-step execution makes little sense with the current semantics... *)
-Definition stmt_multi_exec:
+Definition stmt_multi_exec_def:
  (stmt_multi_exec _ state 0 =
   SOME state)
  /\
@@ -2210,7 +2204,7 @@ End
 (*  Frame list semantics  *)
 (**************************)
 
-Definition frames_exec:
+Definition frames_exec_def:
  (******************************************)
  (* Catch-all clauses for special statuses *)
  (frames_exec (ctx:'a ctx) ((ascope:'a, g_scope_list:g_scope_list, frame_list:frame_list, status_returnv v):'a state) = NONE)
@@ -2363,7 +2357,7 @@ QED
 
 (* TODO: Outsource the stuff that causes too many case splits to other functions
  *       i.e. exec_arch_e, exec_arch_update_return_frame, exec_arch_assign, ... *)
-val arch_exec_def = Define `
+Definition arch_exec_def:
  (arch_exec ((ab_list, pblock_map, ffblock_map, input_f, output_f, copyin_pbl, copyout_pbl, apply_table_f, ext_map, func_map):'a actx)
             (((i, in_out_list, in_out_list', scope):'a aenv), g_scope_list:g_scope_list, arch_frame_list_regular frame_list, status:status) =
   (case EL i ab_list of
@@ -2463,10 +2457,10 @@ val arch_exec_def = Define `
  )
 /\
 (arch_exec _ _ = NONE)
-`;
+End
 
 (* Fuel-powered multi-step architectural-level executable semantics *)
-val arch_multi_exec = Define `
+Definition arch_multi_exec_def:
  (arch_multi_exec actx (aenv, g_scope_list, arch_frame_list, status) 0 =
   SOME (aenv, g_scope_list, arch_frame_list, status))
   /\
@@ -2475,7 +2469,7 @@ val arch_multi_exec = Define `
   | SOME (aenv', g_scope_list', arch_frame_list', status') =>
    arch_multi_exec actx (aenv', g_scope_list', arch_frame_list', status') fuel
   | NONE => NONE)
-`;
+End
 
 Theorem arch_multi_exec_1:
 !actx s s'.
@@ -2483,7 +2477,7 @@ Theorem arch_multi_exec_1:
 Proof
 rpt strip_tac >>
 PairCases_on ‘s’ >>
-REWRITE_TAC [arithmeticTheory.ONE, arch_multi_exec] >>
+REWRITE_TAC [arithmeticTheory.ONE, arch_multi_exec_def] >>
 Cases_on ‘arch_exec actx ((s0,s1,s2,s3),s4,s5,s6)’ >> (
  fs[]
 ) >>
@@ -2500,10 +2494,10 @@ arch_multi_exec actx (aenv, g_scope_list, arch_frame_list, status) (m+n) =
  | NONE => NONE
 Proof
 Induct_on `n` >- (
- fs [arch_multi_exec]
+ fs [arch_multi_exec_def]
 ) >>
 rpt strip_tac >>
-fs [arch_multi_exec, arithmeticTheory.ADD_CLAUSES] >>
+fs [arch_multi_exec_def, arithmeticTheory.ADD_CLAUSES] >>
 Cases_on `arch_exec actx (aenv,g_scope_list,arch_frame_list,status)` >> (
  fs []
 ) >>
@@ -2587,6 +2581,30 @@ gs [] >>
 fs [arch_multi_exec_add]
 QED
 
+Theorem arch_multi_exec_comp_n_tl_assl_conj:
+!n m actx assl aenv g_scope_list arch_frame_list status aenv' g_scope_list' arch_frame_list' status' aenv'' g_scope_list'' arch_frame_list'' status''.
+((assl ==> arch_multi_exec actx (aenv, g_scope_list, arch_frame_list, status) n =
+  SOME (aenv', g_scope_list', arch_frame_list', status')) /\
+ (assl ==> arch_multi_exec actx (aenv', g_scope_list', arch_frame_list', status') m =
+  SOME (aenv'', g_scope_list'', arch_frame_list'', status''))) ==>
+(assl ==> arch_multi_exec actx (aenv, g_scope_list, arch_frame_list, status) (n+m) =
+  SOME (aenv'', g_scope_list'', arch_frame_list'', status''))
+Proof
+metis_tac[arch_multi_exec_comp_n_tl_assl]
+QED
+
+Theorem arch_multi_exec_comp_n_tl_assl_conj_nomidassl:
+!n m actx assl aenv g_scope_list arch_frame_list status aenv' g_scope_list' arch_frame_list' status' aenv'' g_scope_list'' arch_frame_list'' status''.
+((assl ==> arch_multi_exec actx (aenv, g_scope_list, arch_frame_list, status) n =
+  SOME (aenv', g_scope_list', arch_frame_list', status')) /\
+ (arch_multi_exec actx (aenv', g_scope_list', arch_frame_list', status') m =
+  SOME (aenv'', g_scope_list'', arch_frame_list'', status''))) ==>
+(assl ==> arch_multi_exec actx (aenv, g_scope_list, arch_frame_list, status) (n+m) =
+  SOME (aenv'', g_scope_list'', arch_frame_list'', status''))
+Proof
+metis_tac[arch_multi_exec_comp_n_tl_assl_conj]
+QED
+
 Theorem arch_multi_exec_arch_frame_list_regular:
 !ab_list pblock_map ffblock_map input_f output_f copyin_pbl
  copyout_pbl apply_table_f ext_map func_map aenv g_scope_list g_scope_list' arch_frame_list frame_list' n i io_list io_list' ascope.
@@ -2616,7 +2634,7 @@ Cases_on ‘arch_multi_exec
 PairCases_on ‘x’ >>
 fs[] >>
 FULL_SIMP_TAC pure_ss [Once arithmeticTheory.ONE] >>
-fs[arch_multi_exec] >>
+fs[arch_multi_exec_def] >>
 Cases_on ‘x5’ >- (
  Cases_on ‘x6’ >> (
   fs[arch_exec_def]
@@ -2751,7 +2769,7 @@ QED
 
 (*
 (* TODO: some kind of (multi-step) CakeML-adjusted executable semantics definition *)
-Definition e_exec_cake:
+Definition e_exec_cake_def:
  (e_exec_cake (e_unop unop_neg (e_v (v_bool b))) stacks status =
    SOME (e_v (v_bool ~b)))
   /\
